theories/aneris_lang/lib/network_util.v
@@ -1,6 +1,7 @@
 From aneris.aneris_lang Require Import lang tactics proofmode notation.
-From aneris.aneris_lang.lib Require Import assert list map.
+From aneris.aneris_lang.lib Require Import assert list map pers_socket_proto.
 From iris_string_ident Require Import ltac2_string_ident.
+
 Set Default Proof Using "Type".
 
 Definition unSOME : base_lang.val :=
@@ -17,14 +18,14 @@ Definition sendto_all : base_lang.val :=
   λ: "socket" "ns" "msg",
   list_iter (λ: "n", SendTo "socket" "msg" "n") "ns".
 
-Definition receivefrom_all : base_lang.val :=
+Definition receivefrom_all : val :=
   λ: "socket" "nodes",
   letrec: "recv" "n" :=
     let: "msg" := unSOME (ReceiveFrom "socket") in
     let: "sender" := Snd "msg" in
-    if: "sender" = "n" then "msg"
+    if: "sender" = "n" then (Fst "msg")
     else "recv" "n" in
-  list_fold  (λ: "acc" "n", "recv" "n" :: "acc") [] "nodes".
+  list_fold  (λ: "acc" "n", list_append "acc" ["recv" "n"]) [] "nodes".
 
 Import Network.
 
@@ -38,21 +39,74 @@ Section library.
     wp_lam. wp_match. by iApply "HΦ".
   Qed.
 
-  Lemma wp_receivefrom_all nodes φ ns h s a R T :
-    let ip := ip_of_address a in
-    {{{ a ⤇ φ
-          ∗ ⌜is_list (map (LitV ∘ LitSocketAddress) nodes) ns⌝
-          ∗ h ↪[ip] s
-          ∗ a ⤳ (R, T) }}}
+  Lemma wp_receivefrom_all nodes φ ns h s ip a R T :
+    ip = ip_of_address a →
+    saddress s = Some a →
+    sblock s = true →
+    {{{ ⌜is_list (map (LitV ∘ LitSocketAddress) nodes) ns⌝ ∗
+        h ↪[ip] s ∗
+        a ⤇ φ ∗
+        a @ φ ⤳# (R, T) }}}
       receivefrom_all #(LitSocket h) ns @[ip]
     {{{ vs msgs R', RET vs;
         h ↪[ip] s
-          ∗ a ⤳ (R', T) 
-          ∗ ⌜is_list (map (λ m, (#(m_body m), #(m_sender m))%V) msgs) vs⌝
-          ∗ [∗ list] n ∈ nodes, (∃ m, ⌜m ∈ msgs⌝ ∗ ⌜m_sender m = n⌝ ∗ ⌜m ∈ R'⌝ ∗ φ m)  }}}.
+          ∗ a @ φ ⤳# (R', T)
+          ∗ ⌜is_list (map (λ m, #(m_body m)) msgs) vs⌝
+          ∗ [∗ list] n ∈ nodes, (∃ m, ⌜m ∈ msgs⌝ ∗ ⌜m_sender m = n⌝ ∗ φ m) }}}.
   Proof.
-    (* TODO: This does not work; what about duplicate messages??? *)
-    Admitted. 
+    iIntros (Hip ?? Φ) "(Hns & Hh & #Hφ & Ha) HΦ".
+    rewrite /receivefrom_all. wp_pures.
+    wp_apply (wp_list_fold
+                (λ (nodes' : list socket_address) (acc : val), ∃ msgs R,
+                    h ↪[ip] s ∗ a @ φ ⤳# (R, T) ∗
+                      ⌜is_list (map (λ m, #(m_body m)) msgs) acc⌝ ∗
+                      [∗ list] n ∈ nodes', (∃ m, ⌜m ∈ msgs⌝ ∗ ⌜m_sender m = n⌝ ∗ φ m))%I
+                (λ n, True)%I
+                (λ n, True)%I _ _ nodes [] with "[] [$Hns Hh Ha]").
+    - iIntros (n acc lacc lrem Ψ) "!# (% & Hmsgs & _) HΨ".
+      do 3 wp_pure _.
+      wp_bind (((rec: "recv" _ := _)%V _))%E.
+      iLöb as "IH".
+      wp_pures.
+      iDestruct "Hmsgs" as (msgs R') "(Hh & Ha & %Hacc & Hnodes)".
+      wp_apply (aneris_wp_receivefrom_nodup with "[$Hh $Ha $Hφ]"); [done..|].
+      iIntros (m) "(Hh & Ha & Hm)".
+      wp_apply wp_unSOME; [done|]; iIntros "_".
+      wp_pures.
+      case_bool_decide as Heq.
+      + wp_pures.
+        wp_apply wp_list_singleton; [done|].
+        iIntros (??).
+        wp_apply wp_list_append; [done|].
+        iIntros (??).
+        iApply "HΨ". iSplit; [|done].
+        iExists (msgs ++ [m]), _. iFrame.
+        iSplit.
+        { rewrite map_app //. }
+        rewrite big_sepL_app big_sepL_singleton.
+        iSplitL "Hnodes".
+        { iApply (big_sepL_impl with "Hnodes").
+          iIntros "!#" (???).
+          iDestruct 1 as (?) "(% & % & ?)".
+          iExists _. iFrame. simplify_eq.
+          iSplit; [|done].
+          iPureIntro; set_solver. }
+        iExists m. iFrame.
+        inversion_clear Heq.
+        iSplit; [|done].
+        iPureIntro; set_solver.
+      + wp_if.
+        iApply ("IH" with "[-HΨ]").
+        { iExists _, _. by iFrame. }
+        iIntros (?) "[Hmsgs _]".
+        iDestruct "Hmsgs" as (msgs' R'') "(Hh & Ha & %Hmsgs' & Hnodes)".
+        iApply "HΨ".
+        iFrame. iExists _, _. by iFrame.
+    - rewrite big_sepL_emp. iFrame. iExists [], R. iFrame; auto.
+    - iIntros (?) "[Hmsgs _]".
+      iDestruct "Hmsgs" as (msgs R') "(Hh & Ha & %Hmsgs & Hnodes)".
+      iApply "HΦ". by iFrame.
+  Qed.
 
   Lemma wp_sendto_all f m a h s R T ns nodes :
     let ip := ip_of_address a in
@@ -63,18 +117,20 @@ Section library.
           ∗ ⌜is_list (map (LitV ∘ LitSocketAddress) nodes) ns⌝
           ∗ [∗ list] n ∈ nodes, (n ⤇ f n ∗ f n (msg n)) }}}
       sendto_all #(LitSocket h) ns #m @[ip]
-    {{{ R' T', RET #(); h ↪[ip] s ∗ a ⤳ (R', T') ∗ ⌜∀ n, n ∈ nodes → msg n ∈ T'⌝ }}}.
+    {{{ T', RET #(); h ↪[ip] s ∗ a ⤳ (R, T') }}}.
   Proof.
     iIntros (??? Φ) "(Hh & Ha & %Hns & Hnodes) HΦ".
     rewrite /sendto_all. wp_pures.
     wp_apply ((wp_list_iter (λ n, n ⤇ f n ∗ f n (msg n))
                             (λ n, True)
-                            (h ↪[ip] s ∗ ∃ R T, a ⤳ (R, T)) with "[] [$Hnodes $Hh Ha]")%I); [|eauto|].
-    { iIntros (n Ψ)" !# (%Hn & [Hh Ha] & #Hφ & Hmsg) H". iDestruct "Ha" as (R' T') "Ha".
+                            (h ↪[ip] s ∗ ∃ T, a ⤳ (R, T)) with "[] [$Hnodes $Hh Ha]")%I); [|eauto|].
+    { iIntros (n Ψ)" !# (%Hn & [Hh Ha] & #Hφ & Hmsg) H". iDestruct "Ha" as (T') "Ha".
       wp_pures.
       wp_send "Hmsg"; [rewrite /msg //|].
       iApply "H". iFrame. eauto. }
-    iIntros "(Hh & Ha)".
-  Admitted.
+    iIntros "([Hh Ha] & _)".
+    iDestruct "Ha" as (?) "Ha".
+    iApply "HΦ". iFrame.
+  Qed.
 
 End library.
